WIP

Parametricity/Basic.lean
@@ -1,3 +1,5 @@
+import Mathlib.Data.Set.Basic
+
 namespace Parametricity
 
 -- simple types:
@@ -20,58 +22,55 @@ inductive Exp' (ρ : Ty → Type) : Ty → Type where
   | lam (dom : Ty) (body : ρ dom → Exp' ρ cod) : Exp' ρ (.fn dom cod)
 def Exp (ty : Ty) := ∀{ρ : Ty → Type}, Exp' ρ ty
 
-def Exp.interp : Exp Ty.interp ty → ty.interp
+def Exp'.interp {ty : Ty} : Exp' Ty.interp ty → ty.interp
   | .var x => x
   | .unit => ()
   | .boolLit b => b
-  | .app f x => f.interp (x.interp)
-  | .lam dom body => fun x => body x.interp
+  | .app f x => f.interp x.interp
+  | .lam dom body => fun x => (body x).interp
 end SimpleTypes
 
 -- System Fω types:
-namespace SystemF
+namespace SystemFProp
 
-inductive Ki : Type where
-  | star : Ki
-  | arrow (dom : Ki) (cod : Ki) : Ki
+inductive Ty' (ρ : Type u) : Type u where
+  | var (x : ρ) : Ty' ρ
+  | unit : Ty' ρ
+  | bool : Ty' ρ
+  | fn (dom : Ty' ρ) (cod : Ty' ρ) : Ty' ρ
+  | forall (body : ρ → Ty' ρ) : Ty' ρ
+--  | abs (body : Ξ dom → Ty' Ξ ran) : Ty' Ξ (.arrow dom ran)
+--  | app (f : Ty' Ξ (.arrow dom ran)) (x : Ty' Ξ dom) : Ty' Ξ ran
+def Ty : Type (u + 1) := ∀{ρ}, Ty' ρ
 
-def Ki.interp : Ki → Type 1
-  | .star => Type
-  | .arrow dom cod => dom.interp → cod.interp
+def Set.fn (dom : Set Type) (cod : Set Type) : Set Type :=
+  { f | ∃ d c, f = (d → c) ∧ d ∈ dom ∧ c ∈ cod }
 
-inductive Ty' (Ξ : Ki → Type u) : Ki → Type u where
-  | var (x : Ξ ki) : Ty' Ξ ki
-  | unit : Ty' Ξ .star
-  | bool : Ty' Ξ .star
-  | fn (dom : Ty' Ξ .star) (cod : Ty' Ξ .star) : Ty' Ξ .star
-  | forall (body : Ξ .star → Ty' Ξ .star) : Ty' Ξ .star
-  | abs (body : Ξ dom → Ty' Ξ ran) : Ty' Ξ (.arrow dom ran)
-  | app (f : Ty' Ξ (.arrow dom ran)) (x : Ty' Ξ dom) : Ty' Ξ ran
-def Ty (ki : Ki) : Type (u + 1) := ∀{Ξ}, Ty' Ξ ki
+def Set.forall (body : Set Type → Set Type) : Set Type :=
+  { f | ∃ x, f ∈ body x }
 
-def Ty'.interp : Ty' Ki.interp ki → ki.interp
+@[reducible, simp]
+def Ty'.interp : Ty' (Set Type) → Set Type
   | .var x => x
-  | .unit => Unit
-  | .bool => Bool
-  | .fn dom cod => dom.interp → cod.interp
-  | .forall body => ∀ x, (body x).interp
-  | .abs body => fun x => (body x).interp
-  | .app f x => f.interp x.interp
+  | .unit => {Unit}
+  | .bool => {Bool}
+  | .fn dom cod => Set.fn dom.interp cod.interp
+  | .forall body => Set.forall (fun x => (body x).interp)
 
 set_option hygiene false in
 notation τ₁ "[" τ₂ "]↦ " τ₃ => RelSubst τ₁ τ₂ τ₃
-inductive RelSubst : {Ξ : Ki → Type 1} → {ki₁ : Ki} → {ki₂ : Ki} → (Ξ ki₁ → Ty' Ξ ki₂) → Ty' Ξ ki₁ → Ty' Ξ ki₂ → Prop where
+inductive RelSubst : {α : Type u} → (α → Ty' α) → Ty' α → Ty' α → Prop where
   | id : .var [τ]↦ τ
   | var : (fun _ => .var x)[τ]↦ (.var x)
   | bool : (fun _ => .bool)[τ]↦ .bool
   | unit : (fun _ => .unit)[τ]↦ .unit
   | fn (dom : τ₁[τ]↦ τ₁') (ran : τ₂[τ]↦ τ₂')
     : (fun α => .fn (τ₁ α) (τ₂ α))[τ]↦ .fn τ₁' τ₂'
-  | forall {τ₁ : Ξ ki → Ξ dom → Ty' Ξ ran} {τ₁' : Ξ dom → Ty' Ξ ran}
-           (body : ∀ α', RelSubst (ki₁:=ki) (fun α => τ₁ α α') τ (τ₁' α'))
-    : RelSubst (ki₁ := ki) (fun α => .forall (τ₁ α)) τ (.forall τ₁')
+  | forall {τ₁ : α → α → Ty' α} {τ₁' : α → Ty' α}
+           (body : ∀ α', RelSubst (fun α => τ₁ α α') τ (τ₁' α'))
+    : RelSubst (fun α => .forall (τ₁ α)) τ (.forall τ₁')
 
-class RelSubst2 {Ξ : Ki → Type 1} {ki₁ : Ki} {ki₂ : Ki} (τ₁ : Ξ ki₁ → Ty' Ξ ki₂) (τ₂ : Ty' Ξ ki₁) (τ' : outParam (Ty' Ξ ki₂)) where
+class RelSubst2 {α : Type u} (τ₁ : α → Ty' α) (τ₂ : Ty' α) (τ' : outParam (Ty' α)) where
   subst : τ₁[τ₂]↦ τ'
 
 instance : RelSubst2 .var τ τ where
@@ -90,26 +89,66 @@ instance [dom : RelSubst2 τ₁ τ τ₁'] [ran : RelSubst2 τ₂ τ τ₂'] :
   RelSubst2 (fun α => Ty'.fn (τ₁ α) (τ₂ α)) τ (.fn τ₁' τ₂') where
   subst := RelSubst.fn dom.subst ran.subst
 
-instance (τ₁ : Ξ ki → Ξ dom → Ty' Ξ ran) (τ₁' : Ξ dom → Ty' Ξ ran)
-  [body : ∀ α', RelSubst2 (ki₁:=ki) (fun α => τ₁ α α') τ (τ₁' α')] :
+instance (τ₁ : α → α → Ty' α) (τ₁' : α → Ty' α)
+  [body : ∀ α', RelSubst2 (fun α => τ₁ α α') τ (τ₁' α')] :
   RelSubst2 (fun α => Ty'.forall (τ₁ α)) τ (.forall τ₁') where
   subst := RelSubst.forall (fun α => (body α).subst)
 
 -- def RelSubst.f : ∀{ki₁ ki₂ : Ki} {Ξ : Ki → Type} (τ₁ : Ξ ki₁ → Ty' Ξ ki₂) (τ₂ : Ty' Ξ ki₁) ,
 
-inductive Exp' (Ξ : Ki → Type 1) (Γ : (ki:Ki) → Ty' Ξ ki → ki.interp) : {ki:Ki} → Ty' Ξ ki → Type 1 where
-  | var (x : Γ .star ty) : Exp' Ξ Γ ty
-  | unit : Exp' Ξ Γ .unit
-  | boolLit (b : Bool) : Exp' Ξ Γ .bool
-  | app (f : Exp' Ξ Γ (.fn dom cod)) (x : Exp' Ξ Γ dom) : Exp' Ξ Γ cod
-  | abs (dom : Ty' Ξ .star) (body : Γ .star dom → Exp' Ξ Γ cod) : Exp' Ξ Γ (.fn dom cod)
-  | tyabs (dom : Ki) {τ : Ξ dom → Ty' Ξ ran} (body : (x : Ξ dom) → Exp' Ξ Γ (τ x))
-    : Exp' Ξ Γ (.forall τ)
-  | tyapp {τ₁ : Ξ dom → Ty' Ξ ran}
-          (e : Exp' Ξ Γ (.forall τ₁)) (τ₂ : Ty' Ξ dom) (subst : RelSubst τ₁ τ₂ τ')
-    : Exp' Ξ Γ τ'
+abbrev Elem (ty : Set Type) := ∀ τ, τ ∈ ty → Set τ -- ∀ (τ : Subtype ty), τ.val → Prop
+def Elem.mem (x : α) {ty : Set Type} (s : Elem ty) : Prop := ∃ h : α ∈ ty, s α h x
+open Classical in
+def Elem.singleton {ty : Set Type} (x : α) : Elem ty := fun τ _ y => if h : τ = α then h ▸ x = y else False
+def Elem.app {dom cod : Set Type} (f : Elem (Set.fn dom cod)) (a : Elem dom) : Elem cod := fun τ _ =>
+  { efa | ∀ τ' (hf : (τ' → τ) ∈ (Set.fn dom cod)) (ha : τ' ∈ dom)
+          ef ea (hef : ef ∈ f (τ' → τ) hf) (hea : ea ∈ a τ' ha),
+          ef ea = efa }
+def Elem.abs {dom cod : Set Type} (body : Elem dom → Elem cod) : Elem (Set.fn dom cod) := fun τ _ =>
+  { efn | ∀ τ₁ τ₂ (h : τ = (τ₁ → τ₂)) (hτ₁ : τ₁ ∈ dom) (hτ₂ : τ₂ ∈ cod),
+          ∀ (ea : τ₁), body (Elem.singleton ea) τ₂ hτ₂ (cast h efn ea) }
+def Elem.tyapp (f : Elem (Set.forall body)) (a : Set Type) : Elem (body a) := fun τ _ =>
+  { efa | ∀ τ' (hf : (τ' → τ) ∈ (Set.fn dom cod)) (ha : τ' ∈ dom)
+          ef ea (hef : ef ∈ f (τ' → τ) hf) (hea : ea ∈ a τ' ha),
+          ef ea = efa }
 
-def Exp (ki : Ki) (ty : Ty ki) := ∀ {Ξ : Ki → Type 1} {Γ : (ki : Ki) → Ty' Ξ ki → ki.interp}, Exp' Ξ Γ ty
+example : Elem.app (dom := {Unit}) (Elem.abs (fun x => x)) (Elem.singleton ()) Unit (by rfl) () := by
+  simp[Elem.abs, Elem.app]
+  trivial
+
+example : Elem.app (dom := {Unit}) (Elem.abs (fun x => x)) (Elem.singleton ()) Unit (by rfl) () := by
+  simp[Elem.abs, Elem.app]
+  trivial
+
+notation "€" => Elem.mem
+
+inductive Exp' {ρ : Type u} (Γ : Ty' ρ → Type 1) : Ty' ρ → Type (max 1 u) where
+--  | var (x : Elem (Γ ty)) : Exp' Γ ty
+  | var (x : Γ ty) : Exp' Γ ty
+  | unit : Exp' Γ .unit
+  | boolLit (b : Bool) : Exp' Γ .bool
+  | app (f : Exp' Γ (.fn dom cod)) (x : Exp' Γ dom) : Exp' Γ cod
+  | abs (dom : Ty' ρ) (body : Γ dom → Exp' Γ cod) : Exp' Γ (.fn dom cod)
+  | tyabs {τ : ρ → Ty' ρ} (body : (x : ρ) → Exp' Γ (τ x))
+    : Exp' Γ (.forall τ)
+  | tyapp (τ₁ : ρ → Ty' ρ) (e : Exp' Γ (.forall τ₁)) (τ₂ : ρ)
+    : Exp' Γ (τ₁ τ₂)
+
+-- def Exp {ρ : Type u} (ty : Ty) := ∀ {Γ : Ty' ρ → Type u}, Exp' Γ ty
+
+def Ty'.apply ()
+
+open Classical in
+@[reducible]
+def Exp'.interp {ty : Ty' (Set Type)} : Exp' (Elem ∘ Ty'.interp) ty → Elem (Ty'.interp ty)
+  | .var x => x
+  | .unit => Elem.singleton ()
+  | .boolLit b => Elem.singleton b
+  | .app f x => Elem.app f.interp x.interp
+  | .abs dom body => Elem.abs (fun x => (body x).interp)
+  | .tyapp scheme f τ => Elem.tyapp f.interp τ
+--  | .tyabs body => fun x => (body x).interp
+  | _ => sorry
 
 declare_syntax_cat systemf_kind
 syntax:max "[ki|" systemf_kind "|]" : term
@@ -119,9 +158,9 @@ syntax:50 systemf_kind:51 " → " systemf_kind:50 : systemf_kind
 macro_rules
   | `([ki|($k)|]) => `([ki|$k|])
   | `([ki|⋆|]) => `(Ki.star)
-  | `([ki| $k₁ → $k₂ |]) => `(Ki.arrow [ki|$k₁|] [ki|$k₂|])
+-- | `([ki| $k₁ → $k₂ |]) => `(Ki.arrow [ki|$k₁|] [ki|$k₂|])
 
-#check [ki|(⋆ → ⋆) → ⋆ → ⋆|]
+-- #check [ki|(⋆ → ⋆) → ⋆ → ⋆|]
 
 declare_syntax_cat systemf_type
 syntax:max "[ty|" systemf_type " |]" : term
@@ -142,13 +181,13 @@ macro_rules
   | `([ty| $f $x |]) => `(Ty'.app [ty|$f|] [ty|$x|])
   | `([ty| $ty₁ → $ty₂ |]) => `(Ty'.fn [ty|$ty₁|] [ty|$ty₂|])
   | `([ty|∀ $x, $ty|]) => `(Ty'.forall (fun $x => [ty|$ty|]))
-  | `([ty|∀ $x : $ki, $ty|]) => `(Ty'.forall (dom := [ki|$ki|]) (fun $x => [ty|$ty|]))
+  | `([ty|∀ $x : $_ki, $ty|]) => `(Ty'.forall (fun $x => [ty|$ty|]))
 
 #check [ty|(Bool → Unit) → Unit → Bool|]
 #check [ty|∀ x, x |]
 #check [ty|∀ x : ⋆, x |]
-#check [ty|∀ x : ⋆ → ⋆, x Unit |]
-#check [ty|∀ x : ⋆ → ⋆ → ⋆, x Unit Bool |]
+-- #check [ty|∀ x : ⋆ → ⋆, x Unit |]
+-- #check [ty|∀ x : ⋆ → ⋆ → ⋆, x Unit Bool |]
 
 declare_syntax_cat systemf_term
 syntax:max "[exp| " systemf_term " |]" : term
@@ -175,25 +214,249 @@ macro_rules
   | `(systemf_term|λ$x, $e) => `(Exp'.abs _ (fun $x => [exp|$e|]))
   | `(systemf_term|λ$x : $ty, $e) => `(Exp'.abs [ty|$ty|] (fun $x => [exp|$e|]))
   | `(systemf_term|$f $a) => `(Exp'.app [exp|$f|] [exp|$a|])
-  | `(systemf_term|Λ$x, $e) => `(Exp'.tyabs _ (fun $x => [exp|$e|]))
-  | `(systemf_term|Λ$x : $ki, $e) => `(Exp'.tyabs [ki|$ki|] (fun $x => [exp|$e|]))
-  | `(systemf_term|$f[$ty]) => `(Exp'.tyapp [exp|$f|] [ty|$ty|] (RelSubst2.subst))
+  | `(systemf_term|Λ$x, $e) => `(Exp'.tyabs (fun $x => [exp|$e|]))
+  | `(systemf_term|Λ$x : $_ki, $e) => `(Exp'.tyabs (fun $x => [exp|$e|]))
+  | `(systemf_term|$f[$ty]) => `(Exp'.tyapp [exp|$f|] [ty|$ty|] (RelSubst2.subst)) -- tODO fix
 
 #check [exp| () |]
 #check [exp| (λ x, x) |]
 #check [exp| (λ x : Unit, x) |]
 #check [exp| (Λ α, λ x : α, x) |]
-#check [exp| (Λ α, λ x : α, x)[Unit] () |]
+-- #check [exp| (Λ α : ⋆, λ x : α, x)[Unit] () |]
 
-example : Exp .star .unit := [exp| (Λ α, λ x : α, x)[Unit] () |]
+-- example : Exp' Ty'.interp0 .unit := [exp| (Λ α : ⋆, λ x : α, x)[Unit] () |]
 
-def Exp'.interp {ty : Ty' Ki.interp .star} : Exp' Ki.interp @Ty'.interp ty → Ty'.interp ty
+end SystemFProp
+
+-- System Fω types:
+namespace SystemF
+
+inductive Ki : Type u where
+  | star : Ki
+--  | arrow (dom : Ki) (cod : Ki) : Ki
+
+--def Ki.up : Ki.{u} → Ki.{max u v}
+--  | .star => .star
+
+--def Ki.interp : Ki → Type (u + 1)
+--  | .star => Type u
+--  | .arrow dom cod => dom.interp → cod.interp
+
+--def Ki.interp_up : (ki : Ki) → Ki.interp.{u} ki → Ki.interp.{max u v} ki.up
+--  | .star, x => ULift.{max u v} x
+--  | .arrow dom cod, f => fun x => Ki.interp_up cod (f x)
+
+--theorem Ki.interp_ulift.{u} (ki : Ki) : ULift (Ki.interp.{u} ki) = Ki.interp.{u+1} ki := by
+--  intro ki
+--  induction ki
+--  case star =>
+--    rfl
+--  case arrow dom cod ihDom ihCod =>
+--    rw [←ihDom]
+
+inductive Ty' (ρ : Type u) : Type u where
+  | var (x : ρ) : Ty' ρ
+  | unit : Ty' ρ
+  | bool : Ty' ρ
+  | fn (dom : Ty' ρ) (cod : Ty' ρ) : Ty' ρ
+  | forall (body : ρ → Ty' ρ) : Ty' ρ
+--  | abs (body : Ξ dom → Ty' Ξ ran) : Ty' Ξ (.arrow dom ran)
+--  | app (f : Ty' Ξ (.arrow dom ran)) (x : Ty' Ξ dom) : Ty' Ξ ran
+def Ty : Type (u + 1) := ∀{ρ}, Ty' ρ
+
+def Ty'.ULift.pull.{u} {ρ : Type u} : Ty'.{max u v} (ULift ρ) → ULift.{v} (Ty'.{u} ρ)
+  | .var x => .up (.var x.down)
+  | .unit => .up .unit
+  | .bool => .up .bool
+  | .fn dom cod => .up (.fn (Ty'.ULift.pull dom).down (Ty'.ULift.pull cod).down)
+  | .forall body => .up (.forall (fun x => (Ty'.ULift.pull (body (.up x))).down))
+
+def Ty'.ULift.push.{u} {ρ : Type u} (ty : ULift.{v} (Ty' ρ)) : Ty'.{max u v} (ULift ρ) := go ty.down where
+  go : (Ty' ρ) → Ty' (ULift ρ)
+    | .var x => .var (.up x)
+    | .unit => .unit
+    | .bool => .bool
+    | .fn dom cod => .fn (go dom) (go cod)
+    | .forall body => .forall (fun x => go (body x.down))
+
+theorem Ty'.ULift.pull_push {ρ : Type} (ty : Ty'.{u} (ULift ρ)) :
+  Ty'.ULift.push (Ty'.ULift.pull ty) = ty := by
+    induction ty <;> simp_all[push, push.go, pull]
+
+theorem Ty'.ULift.push_pull {ρ : Type} (ty : ULift.{u} (Ty'.{0} ρ)) :
+  Ty'.ULift.pull (Ty'.ULift.push ty) = ty := by
+    cases ty
+    next ty =>
+    induction ty <;> simp_all[pull, push, push.go]
+
+set_option pp.universes true in
+def Ty'.interp.{u} : Ty' (ULift.{u} Type) → ULift.{u} (Type 1)
+  | .var x => .up (ULift x.down)
+  | .unit => .up (ULift Unit)
+  | .bool => .up (ULift Bool)
+  | .fn dom cod => .up (dom.interp.down → cod.interp.down)
+  | .forall body => .up (∀ x, (body (.up x)).interp.down)
+#check Ty'.interp.{0}
+
+def Ty'.interp' : Ty' (Set Type) → Set Type
   | .var x => x
-  | .unit => ⟨⟩
-  | .boolLit b => b
+  | .unit => {Unit}
+  | .bool => {Bool}
+  | .fn dom cod => { f | ∃ d ∈ dom.interp', ∃ c ∈ cod.interp', f = (d → c) }
+  | .forall body => { f | ∃ x, f ∈ (body x).interp' }
+
+def Ty'.interp0 (ty : Ty' Type) : Type 1 :=
+  (Ty'.interp.{0} (Ty'.ULift.push (.up ty))).down
+
+theorem Better.forall_congr {α : Sort u} {p q : α → Sort v} (h : ∀ a, p a = q a) : (∀ a, p a) = (∀ a, q a) :=
+  (funext h : p = q) ▸ rfl
+
+set_option pp.universes true in
+theorem Ty'.interp0_interp {ty : Ty' Type} : Ty'.interp0 ty = (Ty'.interp (Ty'.ULift.push (.up ty))).down := by
+  induction ty <;> simp_all[interp0, interp, ULift.push, ULift.push.go]
+  next ih =>
+  apply Better.forall_congr
+  intro x
+  exact (ih x)
+
+--theorem Ty'.interp_up : Ty'.interp.{u} ty = Ty'.interp.{max u v} (Ty'.up ty) := by
+
+set_option hygiene false in
+notation τ₁ "[" τ₂ "]↦ " τ₃ => RelSubst τ₁ τ₂ τ₃
+inductive RelSubst : {α : Type u} → (α → Ty' α) → Ty' α → Ty' α → Prop where
+  | id : .var [τ]↦ τ
+  | var : (fun _ => .var x)[τ]↦ (.var x)
+  | bool : (fun _ => .bool)[τ]↦ .bool
+  | unit : (fun _ => .unit)[τ]↦ .unit
+  | fn (dom : τ₁[τ]↦ τ₁') (ran : τ₂[τ]↦ τ₂')
+    : (fun α => .fn (τ₁ α) (τ₂ α))[τ]↦ .fn τ₁' τ₂'
+  | forall {τ₁ : α → α → Ty' α} {τ₁' : α → Ty' α}
+           (body : ∀ α', RelSubst (fun α => τ₁ α α') τ (τ₁' α'))
+    : RelSubst (fun α => .forall (τ₁ α)) τ (.forall τ₁')
+
+class RelSubst2 {α : Type u} (τ₁ : α → Ty' α) (τ₂ : Ty' α) (τ' : outParam (Ty' α)) where
+  subst : τ₁[τ₂]↦ τ'
+
+instance : RelSubst2 .var τ τ where
+  subst := RelSubst.id
+
+instance : RelSubst2 (fun _ => Ty'.var x) τ (.var x) where
+  subst := RelSubst.var
+
+instance : RelSubst2 (fun _ => Ty'.bool) τ .bool where
+  subst := RelSubst.bool
+
+instance : RelSubst2 (fun _ => Ty'.unit) τ .unit where
+  subst := RelSubst.unit
+
+instance [dom : RelSubst2 τ₁ τ τ₁'] [ran : RelSubst2 τ₂ τ τ₂'] :
+  RelSubst2 (fun α => Ty'.fn (τ₁ α) (τ₂ α)) τ (.fn τ₁' τ₂') where
+  subst := RelSubst.fn dom.subst ran.subst
+
+instance (τ₁ : α → α → Ty' α) (τ₁' : α → Ty' α)
+  [body : ∀ α', RelSubst2 (fun α => τ₁ α α') τ (τ₁' α')] :
+  RelSubst2 (fun α => Ty'.forall (τ₁ α)) τ (.forall τ₁') where
+  subst := RelSubst.forall (fun α => (body α).subst)
+
+-- def RelSubst.f : ∀{ki₁ ki₂ : Ki} {Ξ : Ki → Type} (τ₁ : Ξ ki₁ → Ty' Ξ ki₂) (τ₂ : Ty' Ξ ki₁) ,
+
+inductive Exp' (Γ : Ty' Type → Type 1) : Ty' Type → Type 1 where
+  | var (x : Γ ty) : Exp' Γ ty
+  | unit : Exp' Γ .unit
+  | boolLit (b : Bool) : Exp' Γ .bool
+  | app (f : Exp' Γ (.fn dom cod)) (x : Exp' Γ dom) : Exp' Γ cod
+  | abs (dom : Ty' Type) (body : Γ dom → Exp' Γ cod) : Exp' Γ (.fn dom cod)
+  | tyabs {τ : Type → Ty' Type} (body : (x : Type) → Exp' Γ (τ x))
+    : Exp' Γ (.forall τ)
+  | tyapp {τ₁ : Type → Ty' Type} (e : Exp' Γ (.forall τ₁)) (τ₂ : Type)
+    : Exp' Γ (τ₁ τ₂)
+
+-- def Exp {ρ : Type u} (ty : Ty) := ∀ {Γ : Ty' ρ → Type u}, Exp' Γ ty
+
+declare_syntax_cat systemf_kind
+syntax:max "[ki|" systemf_kind "|]" : term
+syntax:max "(" systemf_kind ")" : systemf_kind
+syntax:max "⋆" : systemf_kind
+syntax:50 systemf_kind:51 " → " systemf_kind:50 : systemf_kind
+macro_rules
+  | `([ki|($k)|]) => `([ki|$k|])
+  | `([ki|⋆|]) => `(Ki.star)
+-- | `([ki| $k₁ → $k₂ |]) => `(Ki.arrow [ki|$k₁|] [ki|$k₂|])
+
+-- #check [ki|(⋆ → ⋆) → ⋆ → ⋆|]
+
+declare_syntax_cat systemf_type
+syntax:max "[ty|" systemf_type " |]" : term
+syntax:max "(" systemf_type ")" : systemf_type
+syntax:max "Unit" : systemf_type
+syntax:max "Bool" : systemf_type
+syntax:max ident : systemf_type
+syntax:80 systemf_type:80 systemf_type:81 : systemf_type
+syntax:50 systemf_type:51 " → " systemf_type:50 : systemf_type
+syntax:lead "∀" ident ", " systemf_type:20 : systemf_type
+syntax:lead "∀" ident ":" systemf_kind ", " systemf_type:20 : systemf_type
+
+macro_rules
+  | `([ty|($ty)|]) => `([ty|$ty|])
+  | `([ty|Unit|]) => `(Ty'.unit)
+  | `([ty|Bool|]) => `(Ty'.bool)
+  | `([ty| $x:ident |]) => `(Ty'.var $x)
+  | `([ty| $f $x |]) => `(Ty'.app [ty|$f|] [ty|$x|])
+  | `([ty| $ty₁ → $ty₂ |]) => `(Ty'.fn [ty|$ty₁|] [ty|$ty₂|])
+  | `([ty|∀ $x, $ty|]) => `(Ty'.forall (fun $x => [ty|$ty|]))
+  | `([ty|∀ $x : $_ki, $ty|]) => `(Ty'.forall (fun $x => [ty|$ty|]))
+
+#check [ty|(Bool → Unit) → Unit → Bool|]
+#check [ty|∀ x, x |]
+#check [ty|∀ x : ⋆, x |]
+-- #check [ty|∀ x : ⋆ → ⋆, x Unit |]
+-- #check [ty|∀ x : ⋆ → ⋆ → ⋆, x Unit Bool |]
+
+declare_syntax_cat systemf_term
+syntax:max "[exp| " systemf_term " |]" : term
+
+syntax:max "()" : systemf_term
+syntax:max "(" systemf_term ")" : systemf_term
+syntax:max "true" : systemf_term
+syntax:max "false" : systemf_term
+syntax:max ident : systemf_term
+syntax:80 systemf_term:80 systemf_term:81 : systemf_term
+syntax:lead "λ" ident "," systemf_term:20 : systemf_term
+syntax:lead "λ" ident ":" systemf_type "," systemf_term:20 : systemf_term
+syntax:max systemf_term:max "[" systemf_type:max "]" : systemf_term
+syntax:lead "Λ" ident "," systemf_term:20 : systemf_term
+syntax:lead "Λ" ident ":" systemf_kind "," systemf_term:20 : systemf_term
+
+macro_rules
+  | `([exp| $e |]) => `(systemf_term|$e)
+  | `(systemf_term|($e)) => `(systemf_term|$e)
+  | `(systemf_term|()) => `(Exp'.unit)
+  | `(systemf_term|true) => `(Exp'.boolLit Bool.true)
+  | `(systemf_term|false) => `(Exp'.boolLit Bool.false)
+  | `(systemf_term|$x:ident) => `(Exp'.var $x)
+  | `(systemf_term|λ$x, $e) => `(Exp'.abs _ (fun $x => [exp|$e|]))
+  | `(systemf_term|λ$x : $ty, $e) => `(Exp'.abs [ty|$ty|] (fun $x => [exp|$e|]))
+  | `(systemf_term|$f $a) => `(Exp'.app [exp|$f|] [exp|$a|])
+  | `(systemf_term|Λ$x, $e) => `(Exp'.tyabs (fun $x => [exp|$e|]))
+  | `(systemf_term|Λ$x : $_ki, $e) => `(Exp'.tyabs (fun $x => [exp|$e|]))
+  | `(systemf_term|$f[$ty]) => `(Exp'.tyapp [exp|$f|] [ty|$ty|] (RelSubst2.subst)) -- tODO fix
+
+#check [exp| () |]
+#check [exp| (λ x, x) |]
+#check [exp| (λ x : Unit, x) |]
+#check [exp| (Λ α, λ x : α, x) |]
+-- #check [exp| (Λ α : ⋆, λ x : α, x)[Unit] () |]
+
+-- example : Exp' Ty'.interp0 .unit := [exp| (Λ α : ⋆, λ x : α, x)[Unit] () |]
+
+def Exp'.interp {ty : Ty' Type} : Exp' Ty'.interp0 ty → (Ty'.interp.{1} (Ty'.ULift.push (.up ty))).down
+  | .var x => Ty'.interp0_interp ▸ x
+  | .unit => Ty'.interp0_interp ▸ .up ⟨⟩
+  | .boolLit b => Ty'.interp0_interp ▸ .up b
   | .app f x => f.interp x.interp
-  | .abs dom cod => fun x => (cod x).interp
-  | .tyabs dom body => let x := ty; _
---  | .tyapp e τ subst => e.interp τ
+  | .abs dom cod => fun x => (cod (Ty'.interp0_interp ▸ x)).interp
+  | .tyabs body => fun x => (body x).interp
+  | @Exp'.tyapp _ _ _ _ => sorry -- e.interp τ
+  | _ => sorry
 
 end SystemF
